Correctness.thy
@@ -87,24 +87,26 @@ proof -
     (US h\<^sub>u hp\<^sub>u e\<^sub>u ep\<^sub>u vs\<^sub>u 1 sh\<^sub>u 0 0)" by simp
   let ?cd' = "assemble_code ?cd"
   let ?mp = "assembly_map ?cd"
-  let ?mem = "case_register (assm_hp ?cd h\<^sub>u) (assemble_env e\<^sub>u) (assemble_vals vs\<^sub>u) 
-    (assm_stk ?cd sh\<^sub>u)"
+  let ?mem = "case_register (assm_hp ?cd h\<^sub>u hp\<^sub>u) (assemble_env e\<^sub>u ep\<^sub>u) (assemble_vals vs\<^sub>u 1) 
+    (assm_stk ?cd sh\<^sub>u 0)"
   let ?rs = "case_register hp\<^sub>u ep\<^sub>u (Suc 0) 0"
   from R EU have "iter (\<tturnstile> ?cd' \<leadsto>\<^sub>a) 
     (assemble_state ?mp (US nmem 0 nmem 0 nmem 0 (nmem(0 := 0, 1 := 0)) 2 (length ?cd))) 
       (assemble_state ?mp (US h\<^sub>u hp\<^sub>u e\<^sub>u ep\<^sub>u vs\<^sub>u 1 sh\<^sub>u 0 0))" by (metis correcta_iter)
-  hence "iter (\<tturnstile> ?cd' \<leadsto>\<^sub>a) (AS (case_register (assm_hp ?cd nmem) (assemble_env nmem)
-    (assemble_vals nmem) (assm_stk ?cd (nmem(0 := 0, 1 := 0)))) (case_register 0 0 0 2) 0 (Con 0)
-      (length ?cd')) (AS ?mem ?rs 0 (Con 0) 0)" by simp
+  hence "iter (\<tturnstile> ?cd' \<leadsto>\<^sub>a) (AS (case_register (assm_hp ?cd nmem 0) (assemble_env nmem 0)
+    (assemble_vals nmem 0) (assm_stk ?cd (nmem(0 := 0, 1 := 0)) 2)) (case_register 0 0 0 2) 0 
+      (Con 0) (length ?cd')) (AS ?mem ?rs 0 (Con 0) 0)" by simp
   hence "iter (\<tturnstile> disassemble ?cd' \<leadsto>\<^sub>m) 
-    (disassemble_state (AS (case_register (assm_hp ?cd nmem) (assemble_env nmem)
-      (assemble_vals nmem) (assm_stk ?cd (nmem(0 := 0, 1 := 0)))) (case_register 0 0 0 2) 0 (Con 0)
-        (length ?cd'))) (disassemble_state (AS ?mem ?rs 0 (Con 0) 0))" by (metis correctm_iter)
+    (disassemble_state (AS (case_register (assm_hp ?cd nmem 0) (assemble_env nmem 0)
+      (assemble_vals nmem 0) (assm_stk ?cd (nmem(0 := 0, 1 := 0)) 2)) (case_register 0 0 0 2) 0 
+        (Con 0) (length ?cd'))) (disassemble_state (AS ?mem ?rs 0 (Con 0) 0))" 
+    by (metis correctm_iter)
   hence "iter (\<tturnstile> disassemble ?cd' \<leadsto>\<^sub>m) (MS (case_reg 0 1 2 11 0)
-    (unmap_mem (case_register (assm_hp ?cd nmem) (assemble_env nmem) (assemble_vals nmem) 
-      (assm_stk ?cd (nmem(0 := 0, Suc 0 := 0))))) (length ?cd'))
-        (MS (case_reg (4 * hp\<^sub>u) (Suc (4 * ep\<^sub>u)) 6 3 0) (unmap_mem ?mem) 0)" 
+    (unmap_mem (case_register nmem nmem nmem (nmem(0 := (PC, 0), Suc 0 := (Reg Env, 0))))) 
+      (length ?cd')) (MS (case_reg (4 * hp\<^sub>u) (Suc (4 * ep\<^sub>u)) 6 3 0) (unmap_mem ?mem) 0)" 
     by simp
+
+
   with C T have EM: "iter (\<tturnstile> cd \<leadsto>\<^sub>m) (MS (case_reg 0 1 2 11 0) (nmem(3 := 0, 7 := 0)) (length cd)) 
     (MS (case_reg (4 * hp\<^sub>u) (Suc (4 * ep\<^sub>u)) 6 3 0) (unmap_mem ?mem) 0)" by auto
   from EC VT have "print_closure c = print_nexpr (erase v\<^sub>t)" by simp
@@ -118,7 +120,7 @@ proof -
 
 
 
-  have "print_uval (pseudoreg_map \<circ> assemble_heap ?mp h\<^sub>u) (4 * vs\<^sub>u 0) = print_uval h\<^sub>u (vs\<^sub>u 0)" 
+  have "print_uval (pseudoreg_map \<circ> assemble_heap ?mp h\<^sub>u hp\<^sub>u) (4 * vs\<^sub>u 0) = print_uval h\<^sub>u (vs\<^sub>u 0)" 
     by (simp add: assemble_heap_def)
   with PU' have PU: "print_uval (pseudoreg_map \<circ> ?mem Hp) (4 * vs\<^sub>u 0) = print_nexpr (erase v\<^sub>t)" 
     by simp
